<rdf:RDF xmlns:rdf="http://www.w3.org/1999/02/22-rdf-syntax-ns#"
	xmlns:rdfs="http://www.w3.org/2000/01/rdf-schema#"
	xmlns:owl="http://www.w3.org/2002/07/owl#"
	xmlns:vs="http://www.w3.org/2003/06/sw-vocab-status/ns#"
	xmlns:foaf="http://xmlns.com/foaf/0.1/"
	xmlns:dc="http://purl.org/dc/elements/1.1/"
	xmlns:doap="http://usefulinc.com/ns/doap#"
>

<!-- Copyright © 2004-2016 Edd Dumbill <edd@usefulinc.com>
                 2016-2017 Edd Wilder-James <edd@ewj.me>
                 2018-     The DOAP Authors (see AUTHORS file)

   Licensed under the Apache License, Version 2.0 (the "License");
   you may not use this file except in compliance with the License.
   You may obtain a copy of the License at

       http://www.apache.org/licenses/LICENSE-2.0

   Unless required by applicable law or agreed to in writing, software
   distributed under the License is distributed on an "AS IS" BASIS,
   WITHOUT WARRANTIES OR CONDITIONS OF ANY KIND, either express or implied.
   See the License for the specific language governing permissions and
   limitations under the License.

-->

<!-- about this schema -->

<owl:Ontology rdf:about="http://usefulinc.com/ns/doap#">
	<owl:imports rdf:resource="http://xmlns.com/foaf/0.1/index.rdf" />

	<dc:title>Description of a Project (DOAP) vocabulary</dc:title>
	<dc:title xml:lang="zh-CN">项目描述（DOAP）词汇集</dc:title>
	<dc:description>The Description of a Project (DOAP) vocabulary, described using W3C RDF Schema and the Web Ontology Language.</dc:description>
	<dc:description xml:lang="fr">Le vocabulaire Description Of A Project (DOAP, Description D'Un Projet),
		décrit en utilisant RDF Schema du W3C et OWL.</dc:description>
	<dc:description xml:lang="es">El vocabulario Description of a Project (DOAP, Descripción de un Proyecto), descrito usando RDF Schema de W3C
		y Web Ontology Language.</dc:description>
	<dc:description xml:lang="de">Das Vokabular "Description of a Project (DOAP)", beschrieben durch W3C RDF Schema and the Web Ontology Language.</dc:description>
	<dc:description xml:lang="cs">Slovník Description of a Project (DOAP, Popis projektu), popsaný použitím W3C RDF Schema a Web Ontology Language.</dc:description>
	<dc:description xml:lang="pt">Vocabulário de descrição de um Projeto (DOAP - Description of a Project), descrito no esquema (schema) W3C RDF e na Web Ontology Language.</dc:description>
	<dc:description xml:lang="zh-CN">项目描述（DOAP）词汇集使用了W3C的RDF和网络本体语义进行描述。</dc:description>
	<dc:creator>Edd Wilder-James</dc:creator>
	<dc:format>application/rdf+xml</dc:format>
	<dc:rights>Copyright © The DOAP Authors</dc:rights>

	<foaf:maker>
		<foaf:Person>
			<foaf:name>Edd Wilder-James</foaf:name>
			<foaf:mbox rdf:resource="mailto:edd@usefulinc.com" />
		</foaf:Person>
	</foaf:maker>

</owl:Ontology>

<!-- Classes are listed first -->

<rdfs:Class rdf:about="http://usefulinc.com/ns/doap#Project">
	<rdfs:isDefinedBy rdf:resource="http://usefulinc.com/ns/doap#" />
	<rdfs:label xml:lang="en">Project</rdfs:label>
	<rdfs:label xml:lang="fr">Projet</rdfs:label>
	<rdfs:label xml:lang="es">Proyecto</rdfs:label>
	<rdfs:label xml:lang="de">Projekt</rdfs:label>
	<rdfs:label xml:lang="cs">Projekt</rdfs:label>
	<rdfs:label xml:lang="pt">Projeto</rdfs:label>
	<rdfs:label xml:lang="zh-CN">项目</rdfs:label>
	<rdfs:comment xml:lang="en">A project.</rdfs:comment>
	<rdfs:comment xml:lang="fr">Un projet.</rdfs:comment>
	<rdfs:comment xml:lang="es">Un proyecto.</rdfs:comment>
	<rdfs:comment xml:lang="de">Ein Projekt.</rdfs:comment>
	<rdfs:comment xml:lang="cs">Projekt.</rdfs:comment>
	<rdfs:comment xml:lang="pt">Projeto.</rdfs:comment>
	<rdfs:comment xml:lang="zh-CN">一个项目。</rdfs:comment>
	<rdfs:subClassOf rdf:resource="http://xmlns.com/wordnet/1.6/Project" />
	<rdfs:subClassOf rdf:resource="http://xmlns.com/foaf/0.1/Project" />
</rdfs:Class>

<rdfs:Class rdf:about="http://usefulinc.com/ns/doap#Version">
	<rdfs:isDefinedBy rdf:resource="http://usefulinc.com/ns/doap#" />
	<rdfs:label xml:lang="en">Version</rdfs:label>
	<rdfs:label xml:lang="fr">Version</rdfs:label>
	<rdfs:label xml:lang="es">Versión</rdfs:label>
	<rdfs:label xml:lang="de">Version</rdfs:label>
	<rdfs:label xml:lang="cs">Verze</rdfs:label>
	<rdfs:label xml:lang="pt">Versão</rdfs:label>
	<rdfs:label xml:lang="zh-CN">版本</rdfs:label>
	<rdfs:comment xml:lang="en">Version information of a project release.</rdfs:comment>
	<rdfs:comment xml:lang="fr">Détails sur une version d'une release d'un projet.</rdfs:comment>
	<rdfs:comment xml:lang="es">Información sobre la versión de un release del proyecto.</rdfs:comment>
	<rdfs:comment xml:lang="de">Versionsinformation eines Projekt Releases.</rdfs:comment>
	<rdfs:comment xml:lang="cs">Informace o uvolněné verzi projektu.</rdfs:comment>
	<rdfs:comment xml:lang="pt">Informação sobre a versão do projeto lançado.</rdfs:comment>
	<rdfs:comment xml:lang="zh-CN">项目发布的版本信息。</rdfs:comment>
</rdfs:Class>

<rdfs:Class rdf:about="http://usefulinc.com/ns/doap#Specification">
	<rdfs:isDefinedBy rdf:resource="http://usefulinc.com/ns/doap#" />
	<rdfs:label xml:lang="en">Specification</rdfs:label>
	<rdfs:label xml:lang="pt">Especificação</rdfs:label>
	<rdfs:label xml:lang="zh-CN">规范</rdfs:label>
	<rdfs:comment xml:lang="en">A specification of a system's aspects, technical or otherwise.</rdfs:comment>
	<rdfs:comment xml:lang="pt">A especificação de aspetos, técnicas ou outros do sistema.</rdfs:comment>
	<rdfs:comment xml:lang="zh-CN">有关系统的特性、技术或其它的规范。</rdfs:comment>
	<rdfs:subClassOf rdf:resource="http://www.w3.org/2000/01/rdf-schema#Resource"/>
</rdfs:Class>

<rdfs:Class rdf:about="http://usefulinc.com/ns/doap#Repository">
	<rdfs:isDefinedBy rdf:resource="http://usefulinc.com/ns/doap#" />
	<rdfs:label xml:lang="en">Repository</rdfs:label>
	<rdfs:label xml:lang="fr">Dépôt</rdfs:label>
	<rdfs:label xml:lang="es">Repositorio</rdfs:label>
	<rdfs:label xml:lang="de">Repository</rdfs:label>
	<rdfs:label xml:lang="cs">Úložiště</rdfs:label>
	<rdfs:label xml:lang="pt">Repositório</rdfs:label>
	<rdfs:label xml:lang="zh-CN">仓库</rdfs:label>
	<rdfs:comment xml:lang="en">Source code repository.</rdfs:comment>
	<rdfs:comment xml:lang="fr">Dépôt du code source.</rdfs:comment>
	<rdfs:comment xml:lang="es">Repositorio del código fuente.</rdfs:comment>
	<rdfs:comment xml:lang="de">Quellcode-Versionierungssystem.</rdfs:comment>
	<rdfs:comment xml:lang="cs">Úložiště zdrojových kódů.</rdfs:comment>
	<rdfs:comment xml:lang="pt">Repositório do código fonte.</rdfs:comment>
	<rdfs:comment xml:lang="zh-CN">源代码仓库。</rdfs:comment>
</rdfs:Class>

<rdfs:Class rdf:about="http://usefulinc.com/ns/doap#SVNRepository">
	<rdfs:isDefinedBy rdf:resource="http://usefulinc.com/ns/doap#" />
	<rdfs:label xml:lang="en">Subversion Repository</rdfs:label>
	<rdfs:label xml:lang="fr">Dépôt Subversion</rdfs:label>
	<rdfs:label xml:lang="es">Repositorio Subversion</rdfs:label>
	<rdfs:label xml:lang="de">Subversion Repository</rdfs:label>
	<rdfs:label xml:lang="cs">Úložiště Subversion</rdfs:label>
	<rdfs:label xml:lang="pt">Repositório Subversion</rdfs:label>
	<rdfs:label xml:lang="zh-CN">Subversion仓库</rdfs:label>
	<rdfs:comment xml:lang="en">Subversion source code repository.</rdfs:comment>
	<rdfs:comment xml:lang="fr">Dépôt Subversion du code source.</rdfs:comment>
	<rdfs:comment xml:lang="es">Repositorio Subversion del código fuente.</rdfs:comment>
	<rdfs:comment xml:lang="de">Subversion Quellcode-Versionierungssystem.</rdfs:comment>
	<rdfs:comment xml:lang="cs">Úložiště zdrojových kódů Subversion.</rdfs:comment>
	<rdfs:comment xml:lang="pt">Repositório Subversion do código fonte.</rdfs:comment>
	<rdfs:comment xml:lang="zh-CN">Subversion源代码仓库。</rdfs:comment>
	<rdfs:subClassOf rdf:resource="http://usefulinc.com/ns/doap#Repository" />
</rdfs:Class>

<rdfs:Class rdf:about="http://usefulinc.com/ns/doap#GitRepository">
	<rdfs:isDefinedBy rdf:resource="http://usefulinc.com/ns/doap#" />
	<rdfs:label xml:lang="en">Git Repository</rdfs:label>
	<rdfs:label xml:lang="fr">Dépôt Git</rdfs:label>
	<rdfs:label xml:lang="es">Repositorio Git</rdfs:label>
	<rdfs:label xml:lang="de">Git Repository</rdfs:label>
	<rdfs:label xml:lang="cs">Úložiště Git</rdfs:label>
	<rdfs:label xml:lang="pt">Repositório Git</rdfs:label>
	<rdfs:label xml:lang="zh-CN">Git仓库</rdfs:label>
	<rdfs:comment xml:lang="en">Git source code repository.</rdfs:comment>
	<rdfs:comment xml:lang="fr">Dépôt Git du code source.</rdfs:comment>
	<rdfs:comment xml:lang="es">Repositorio Git del código fuente.</rdfs:comment>
	<rdfs:comment xml:lang="de">Git Quellcode-Versionierungssystem.</rdfs:comment>
	<rdfs:comment xml:lang="cs">Úložiště zdrojových kódů Git.</rdfs:comment>
	<rdfs:comment xml:lang="pt">Repositório Git do código fonte.</rdfs:comment>
	<rdfs:comment xml:lang="zh-CN">Git源代码仓库。</rdfs:comment>
	<rdfs:subClassOf rdf:resource="http://usefulinc.com/ns/doap#Repository" />
</rdfs:Class>

<rdfs:Class rdf:about="http://usefulinc.com/ns/doap#BKRepository">
	<rdfs:isDefinedBy rdf:resource="http://usefulinc.com/ns/doap#" />
	<rdfs:label xml:lang="en">BitKeeper Repository</rdfs:label>
	<rdfs:label xml:lang="fr">Dépôt BitKeeper</rdfs:label>
	<rdfs:label xml:lang="es">Repositorio BitKeeper</rdfs:label>
	<rdfs:label xml:lang="de">BitKeeper Repository</rdfs:label>
	<rdfs:label xml:lang="cs">Úložiště BitKeeper</rdfs:label>
	<rdfs:label xml:lang="pt">Repositório Bitkeeper</rdfs:label>
	<rdfs:label xml:lang="zh-CN">BitKeeper仓库</rdfs:label>
	<rdfs:comment xml:lang="en">BitKeeper source code repository.</rdfs:comment>
	<rdfs:comment xml:lang="fr">Dépôt BitKeeper du code source.</rdfs:comment>
	<rdfs:comment xml:lang="es">Repositorio BitKeeper del código fuente.</rdfs:comment>
	<rdfs:comment xml:lang="de">BitKeeper Quellcode-Versionierungssystem.</rdfs:comment>
	<rdfs:comment xml:lang="cs">Úložiště zdrojových kódů BitKeeper.</rdfs:comment>
	<rdfs:comment xml:lang="pt">Repositório BitKeeper do código fonte.</rdfs:comment>
	<rdfs:comment xml:lang="zh-CN">BitKeeper源代码仓库。</rdfs:comment>
	<rdfs:subClassOf rdf:resource="http://usefulinc.com/ns/doap#Repository" />
</rdfs:Class>

<rdfs:Class rdf:about="http://usefulinc.com/ns/doap#CVSRepository">
	<rdfs:isDefinedBy rdf:resource="http://usefulinc.com/ns/doap#" />
	<rdfs:label xml:lang="en">CVS Repository</rdfs:label>
	<rdfs:label xml:lang="fr">Dépôt CVS</rdfs:label>
	<rdfs:label xml:lang="es">Repositorio CVS</rdfs:label>
	<rdfs:label xml:lang="de">CVS Repository</rdfs:label>
	<rdfs:label xml:lang="cs">Úložiště CVS</rdfs:label>
	<rdfs:label xml:lang="pt">Repositório CVS</rdfs:label>
	<rdfs:label xml:lang="zh-CN">CVS仓库</rdfs:label>
	<rdfs:comment xml:lang="en">CVS source code repository.</rdfs:comment>
	<rdfs:comment xml:lang="fr">Dépôt CVS du code source.</rdfs:comment>
	<rdfs:comment xml:lang="es">Repositorio CVS del código fuente.</rdfs:comment>
	<rdfs:comment xml:lang="de">CVS Quellcode-Versionierungssystem.</rdfs:comment>
	<rdfs:comment xml:lang="cs">Úložiště zdrojových kódů CVS.</rdfs:comment>
	<rdfs:comment xml:lang="pt">Repositório CVS do código fonte.</rdfs:comment>
	<rdfs:comment xml:lang="zh-CN">CVS源代码仓库。</rdfs:comment>
	<rdfs:subClassOf rdf:resource="http://usefulinc.com/ns/doap#Repository" />
</rdfs:Class>

<rdfs:Class rdf:about="http://usefulinc.com/ns/doap#ArchRepository">
	<rdfs:isDefinedBy rdf:resource="http://usefulinc.com/ns/doap#" />
	<rdfs:label xml:lang="en">GNU Arch repository</rdfs:label>
	<rdfs:label xml:lang="fr">Dépôt GNU Arch</rdfs:label>
	<rdfs:label xml:lang="es">Repositorio GNU Arch</rdfs:label>
	<rdfs:label xml:lang="de">GNU Arch repository</rdfs:label>
	<rdfs:label xml:lang="cs">Úložiště GNU Arch</rdfs:label>
	<rdfs:label xml:lang="pt">Repositório GNU Arch</rdfs:label>
	<rdfs:label xml:lang="zh-CN">GNU Arch仓库</rdfs:label>
	<rdfs:comment xml:lang="en">GNU Arch source code repository.</rdfs:comment>
	<rdfs:comment xml:lang="fr">Dépôt GNU Arch du code source.</rdfs:comment>
	<rdfs:comment xml:lang="es">Repositorio GNU Arch del código fuente.</rdfs:comment>
	<rdfs:comment xml:lang="de">GNU Arch Quellcode-Versionierungssystem.</rdfs:comment>
	<rdfs:comment xml:lang="cs">Úložiště zdrojových kódů GNU Arch.</rdfs:comment>
	<rdfs:comment xml:lang="pt">Repositório GNU Arch do código fonte.</rdfs:comment>
	<rdfs:comment xml:lang="zh-CN">GNU Arch源代码仓库。</rdfs:comment>
	<rdfs:subClassOf rdf:resource="http://usefulinc.com/ns/doap#Repository" />
</rdfs:Class>

<rdfs:Class rdf:about="http://usefulinc.com/ns/doap#BazaarBranch">
	<rdfs:isDefinedBy rdf:resource="http://usefulinc.com/ns/doap#" />
	<rdfs:label xml:lang="en">Bazaar Branch</rdfs:label>
	<rdfs:label xml:lang="pt">Ramificação Bazaar</rdfs:label>
	<rdfs:label xml:lang="zh-CN">Bazaar分支</rdfs:label>
	<rdfs:comment xml:lang="en">Bazaar source code branch.</rdfs:comment>
	<rdfs:comment xml:lang="pt">Código fonte da ramificação Bazaar.</rdfs:comment>
	<rdfs:comment xml:lang="zh-CN">源代码的Bazaar分支。</rdfs:comment>
	<rdfs:subClassOf rdf:resource="http://usefulinc.com/ns/doap#Repository" />
</rdfs:Class>

<rdfs:Class rdf:about="http://usefulinc.com/ns/doap#GitBranch">
	<rdfs:isDefinedBy rdf:resource="http://usefulinc.com/ns/doap#" />
	<rdfs:label xml:lang="en">Git Branch</rdfs:label>
	<rdfs:label xml:lang="pt">Ramificação Git</rdfs:label>
	<rdfs:label xml:lang="zh-CN">Git分支</rdfs:label>
	<rdfs:comment xml:lang="en">Git source code branch.</rdfs:comment>
	<rdfs:comment xml:lang="pt">Código fonte da ramificação Git.</rdfs:comment>
	<rdfs:comment xml:lang="zh-CN">源代码的Git分支。</rdfs:comment>
	<rdfs:subClassOf rdf:resource="http://usefulinc.com/ns/doap#Repository" />
</rdfs:Class>

<rdfs:Class rdf:about="http://usefulinc.com/ns/doap#HgRepository">
	<rdfs:isDefinedBy rdf:resource="http://usefulinc.com/ns/doap#" />
	<rdfs:label xml:lang="en">Mercurial Repository</rdfs:label>
	<rdfs:label xml:lang="pt">Repositório Mercurial</rdfs:label>
	<rdfs:label xml:lang="zh-CN">Mercurial仓库</rdfs:label>
	<rdfs:comment xml:lang="en">Mercurial source code repository.</rdfs:comment>
	<rdfs:comment xml:lang="pt">Repositório Mercurial do código fonte.</rdfs:comment>
	<rdfs:comment xml:lang="zh-CN">Mercurial源代码仓库。</rdfs:comment>
	<rdfs:subClassOf rdf:resource="http://usefulinc.com/ns/doap#Repository" />
</rdfs:Class>

<rdfs:Class rdf:about="http://usefulinc.com/ns/doap#DarcsRepository">
	<rdfs:isDefinedBy rdf:resource="http://usefulinc.com/ns/doap#" />
	<rdfs:label xml:lang="en">darcs Repository</rdfs:label>
	<rdfs:label xml:lang="fr">Dépôt darcs</rdfs:label>
	<rdfs:label xml:lang="es">Repositorio darcs</rdfs:label>
	<rdfs:label xml:lang="pt">Repositório darcs</rdfs:label>
	<rdfs:label xml:lang="zh-CN">darcs仓库</rdfs:label>
	<rdfs:comment xml:lang="en">darcs source code repository.</rdfs:comment>
	<rdfs:comment xml:lang="fr">Dépôt darcs du code source.</rdfs:comment>
	<rdfs:comment xml:lang="es">Repositorio darcs del código fuente.</rdfs:comment>
	<rdfs:comment xml:lang="pt">Repositório darcs do código fonte.</rdfs:comment>
	<rdfs:comment xml:lang="zh-CN">darcs源代码仓库。</rdfs:comment>
	<rdfs:subClassOf rdf:resource="http://usefulinc.com/ns/doap#Repository" />
</rdfs:Class>



<!-- Properties -->

<rdf:Property rdf:about="http://usefulinc.com/ns/doap#name">
	<rdfs:isDefinedBy rdf:resource="http://usefulinc.com/ns/doap#" />
	<rdfs:label xml:lang="en">name</rdfs:label>
	<rdfs:label xml:lang="fr">nom</rdfs:label>
	<rdfs:label xml:lang="es">nombre</rdfs:label>
	<rdfs:label xml:lang="de">Name</rdfs:label>
	<rdfs:label xml:lang="cs">jméno</rdfs:label>
	<rdfs:label xml:lang="pt">nome</rdfs:label>
	<rdfs:label xml:lang="zh-CN">名称</rdfs:label>
	<rdfs:comment xml:lang="en">A name of something.</rdfs:comment>
	<rdfs:comment xml:lang="fr">Le nom de quelque chose.</rdfs:comment>
	<rdfs:comment xml:lang="es">El nombre de algo.</rdfs:comment>
	<rdfs:comment xml:lang="de">Der Name von Irgendwas</rdfs:comment>
	<rdfs:comment xml:lang="cs">Jméno něčeho.</rdfs:comment>
	<rdfs:comment xml:lang="pt">O nome de alguma coisa.</rdfs:comment>
	<rdfs:comment xml:lang="zh-CN">某物的名称。</rdfs:comment>
	<rdfs:range rdf:resource="http://www.w3.org/2000/01/rdf-schema#Literal" />
	<rdfs:subPropertyOf rdf:resource="http://www.w3.org/2000/01/rdf-schema#label" />
</rdf:Property>

<rdf:Property rdf:about="http://usefulinc.com/ns/doap#homepage">
	<rdfs:isDefinedBy rdf:resource="http://usefulinc.com/ns/doap#" />
	<rdfs:label xml:lang="en">homepage</rdfs:label>
	<rdfs:label xml:lang="fr">page web</rdfs:label>
	<rdfs:label xml:lang="es">página web</rdfs:label>
	<rdfs:label xml:lang="de">Homepage</rdfs:label>
	<rdfs:label xml:lang="cs">domovská stránka</rdfs:label>
	<rdfs:label xml:lang="pt">página web</rdfs:label>
	<rdfs:label xml:lang="zh-CN">主页</rdfs:label>
	<rdfs:comment xml:lang="en">URL of a project's homepage,
		associated with exactly one project.</rdfs:comment>
	<rdfs:comment xml:lang="fr">L'URL de la page web d'un projet,
		associée avec un unique projet.</rdfs:comment>
	<rdfs:comment xml:lang="es">El URL de la página de un proyecto,
		asociada con exactamente un proyecto.</rdfs:comment>
	<rdfs:comment xml:lang="de">URL der Projekt-Homepage,
		verbunden mit genau einem Projekt.</rdfs:comment>
	<rdfs:comment xml:lang="cs">URL adresa domovské stránky projektu asociované s právě jedním projektem.</rdfs:comment>
	<rdfs:comment xml:lang="pt">O URL da página de um projeto,
		asociada com exactamente um projeto.</rdfs:comment>
	<rdfs:comment xml:lang="zh-CN">确切地关联到一个项目的项目主页URL。</rdfs:comment>
	<rdf:type rdf:resource="http://www.w3.org/2002/07/owl#InverseFunctionalProperty" />
	<rdfs:domain rdf:resource="http://usefulinc.com/ns/doap#Project" />
	<rdfs:subPropertyOf rdf:resource="http://xmlns.com/foaf/0.1/homepage" />
</rdf:Property>

<rdf:Property rdf:about="http://usefulinc.com/ns/doap#old-homepage">
	<rdfs:isDefinedBy rdf:resource="http://usefulinc.com/ns/doap#" />
	<rdfs:label xml:lang="en">old homepage</rdfs:label>
	<rdfs:label xml:lang="fr">ancienne page web</rdfs:label>
	<rdfs:label xml:lang="es">página web antigua</rdfs:label>
	<rdfs:label xml:lang="de">Alte Homepage</rdfs:label>
	<rdfs:label xml:lang="cs">stará domovská stránka</rdfs:label>
	<rdfs:label xml:lang="pt">página web antiga</rdfs:label>
	<rdfs:label xml:lang="zh-CN">旧主页</rdfs:label>
	<rdfs:comment xml:lang="en">URL of a project's past homepage,
		associated with exactly one project.</rdfs:comment>
	<rdfs:comment xml:lang="fr">L'URL d'une ancienne page web d'un
		projet, associée avec un unique projet.</rdfs:comment>
	<rdfs:comment xml:lang="es">El URL de la antigua página de un proyecto,
		asociada con exactamente un proyecto.</rdfs:comment>
	<rdfs:comment xml:lang="de">URL der letzten Projekt-Homepage,
		verbunden mit genau einem Projekt.</rdfs:comment>
	<rdfs:comment xml:lang="cs">URL adresa předešlé domovské stránky projektu asociované s právě jedním projektem.</rdfs:comment>
	<rdfs:comment xml:lang="pt">O URL antigo da página de um projeto,
		associada com exactamente um projeto.</rdfs:comment>
	<rdfs:comment xml:lang="zh-CN">确切地关联到一个项目的项目旧主页URL。</rdfs:comment>
	<rdf:type rdf:resource="http://www.w3.org/2002/07/owl#InverseFunctionalProperty" />
	<rdfs:domain rdf:resource="http://usefulinc.com/ns/doap#Project" />
	<rdfs:subPropertyOf rdf:resource="http://xmlns.com/foaf/0.1/homepage" />
</rdf:Property>

<rdf:Property rdf:about="http://usefulinc.com/ns/doap#security-policy">
	<rdfs:isDefinedBy rdf:resource="http://usefulinc.com/ns/doap#" />
	<rdfs:label xml:lang="en">security policy</rdfs:label>
	<rdfs:comment xml:lang="en">URL of the security policy of a project.</rdfs:comment>
	<rdfs:domain rdf:resource="http://usefulinc.com/ns/doap#Project" />
	<rdfs:subPropertyOf rdf:resource="http://xmlns.com/foaf/0.1/page" />
</rdf:Property>

<rdf:Property rdf:about="http://usefulinc.com/ns/doap#created">
	<rdfs:isDefinedBy rdf:resource="http://usefulinc.com/ns/doap#" />
	<rdfs:label xml:lang="en">created</rdfs:label>
	<rdfs:label xml:lang="fr">créé</rdfs:label>
	<rdfs:label xml:lang="es">creado</rdfs:label>
	<rdfs:label xml:lang="de">erstellt</rdfs:label>
	<rdfs:label xml:lang="cs">vytvořeno</rdfs:label>
	<rdfs:label xml:lang="pt">criado</rdfs:label>
	<rdfs:label xml:lang="zh-CN">创建日期</rdfs:label>
	<rdfs:comment xml:lang="en">Date when something was created, in YYYY-MM-DD form. e.g. 2004-04-05</rdfs:comment>
	<rdfs:comment xml:lang="fr">Date à laquelle a été créé quelque chose, au format AAAA-MM-JJ (par ex. 2004-04-05)</rdfs:comment>
	<rdfs:comment xml:lang="es">Fecha en la que algo fue creado, en formato AAAA-MM-DD. e.g. 2004-04-05</rdfs:comment>
	<rdfs:comment xml:lang="de">Erstellungsdatum von Irgendwas, angegeben im YYYY-MM-DD Format, z.B. 2004-04-05.</rdfs:comment>
	<rdfs:comment xml:lang="cs">Datum, kdy bylo něco vytvořeno ve formátu RRRR-MM-DD, např. 2004-04-05</rdfs:comment>
	<rdfs:comment xml:lang="pt">Data em que algo foi criado, no formato AAAA-MM-DD. e.g. 2004-04-05</rdfs:comment>
	<rdfs:comment xml:lang="zh-CN">某物的创建日期，YYYY-MM-DD格式，比如2004-04-05。</rdfs:comment>
	<rdfs:range rdf:resource="http://www.w3.org/2000/01/rdf-schema#Literal" />
</rdf:Property>

<rdf:Property rdf:about="http://usefulinc.com/ns/doap#shortdesc">
	<rdfs:isDefinedBy rdf:resource="http://usefulinc.com/ns/doap#" />
	<rdfs:label xml:lang="en">short description</rdfs:label>
	<rdfs:label xml:lang="fr">description courte</rdfs:label>
	<rdfs:label xml:lang="es">descripción corta</rdfs:label>
	<rdfs:label xml:lang="de">Kurzbeschreibung</rdfs:label>
	<rdfs:label xml:lang="cs">krátký popis</rdfs:label>
	<rdfs:label xml:lang="pt">descrição curta</rdfs:label>
	<rdfs:label xml:lang="zh-CN">简述</rdfs:label>
	<rdfs:comment xml:lang="en">Short (8 or 9 words) plain text description of a project.</rdfs:comment>
	<rdfs:comment xml:lang="fr">Texte descriptif concis (8 ou 9 mots) d'un projet.</rdfs:comment>
	<rdfs:comment xml:lang="es">Descripción corta (8 o 9 palabras) en texto plano de un proyecto.</rdfs:comment>
	<rdfs:comment xml:lang="de">Kurzbeschreibung (8 oder 9 Wörter) eines Projekts als einfacher Text.</rdfs:comment>
	<rdfs:comment xml:lang="cs">Krátký (8 nebo 9 slov) čistě textový popis projektu.</rdfs:comment>
	<rdfs:comment xml:lang="pt">Descrição curta (com 8 ou 9 palavras) de um projeto em texto apenas.</rdfs:comment>
	<rdfs:comment xml:lang="zh-CN">关于项目的简短文本描述（8或9个单词）。</rdfs:comment>
	<rdfs:range rdf:resource="http://www.w3.org/2000/01/rdf-schema#Literal" />
</rdf:Property>

<rdf:Property rdf:about="http://usefulinc.com/ns/doap#description">
	<rdfs:isDefinedBy rdf:resource="http://usefulinc.com/ns/doap#" />
	<rdfs:label xml:lang="en">description</rdfs:label>
	<rdfs:label xml:lang="fr">description</rdfs:label>
	<rdfs:label xml:lang="es">descripción</rdfs:label>
	<rdfs:label xml:lang="de">Beschreibung</rdfs:label>
	<rdfs:label xml:lang="cs">popis</rdfs:label>
	<rdfs:label xml:lang="pt">descrição</rdfs:label>
	<rdfs:label xml:lang="zh-CN">描述</rdfs:label>
	<rdfs:comment xml:lang="en">Plain text description of a project, of 2-4 sentences in length.</rdfs:comment>
	<rdfs:comment xml:lang="fr">Texte descriptif d'un projet, long de 2 à 4 phrases.</rdfs:comment>
	<rdfs:comment xml:lang="es">Descripción en texto plano de un proyecto, de 2 a 4 enunciados de longitud.</rdfs:comment>
	<rdfs:comment xml:lang="de">Beschreibung eines Projekts als einfacher Text mit der Länge von 2 bis 4 Sätzen.</rdfs:comment>
	<rdfs:comment xml:lang="cs">Čistě textový, 2 až 4 věty dlouhý popis projektu.</rdfs:comment>
	<rdfs:comment xml:lang="pt">Descrição de um projeto em texto apenas, com 2 a 4 frases de comprimento.</rdfs:comment>
	<rdfs:comment xml:lang="zh-CN">关于项目的文本描述，一般是两到四句的长度。</rdfs:comment>
	<rdfs:range rdf:resource="http://www.w3.org/2000/01/rdf-schema#Literal" />
</rdf:Property>

<rdf:Property rdf:about="http://usefulinc.com/ns/doap#release">
	<rdfs:isDefinedBy rdf:resource="http://usefulinc.com/ns/doap#" />
	<rdfs:label xml:lang="en">release</rdfs:label>
	<rdfs:label xml:lang="fr">release</rdfs:label>
	<rdfs:label xml:lang="es">release</rdfs:label>
	<rdfs:label xml:lang="de">Release</rdfs:label>
	<rdfs:label xml:lang="cs">release</rdfs:label>
	<rdfs:label xml:lang="pt">publicação</rdfs:label>
	<rdfs:label xml:lang="zh-CN">发行版</rdfs:label>
	<rdfs:comment xml:lang="en">A project release.</rdfs:comment>
	<rdfs:comment xml:lang="fr">Une release (révision) d'un projet.</rdfs:comment>
	<rdfs:comment xml:lang="es">Un release (versión) de un proyecto.</rdfs:comment>
	<rdfs:comment xml:lang="de">Ein Release (Version) eines Projekts.</rdfs:comment>
	<rdfs:comment xml:lang="cs">Relase (verze) projektu.</rdfs:comment>
	<rdfs:comment xml:lang="pt">A publicação de um projeto.</rdfs:comment>
	<rdfs:comment xml:lang="zh-CN">项目的发行版本。</rdfs:comment>
	<rdfs:domain rdf:resource="http://usefulinc.com/ns/doap#Project" />
	<rdfs:range rdf:resource="http://usefulinc.com/ns/doap#Version" />
</rdf:Property>

<rdf:Property rdf:about="http://usefulinc.com/ns/doap#mailing-list">
	<rdfs:isDefinedBy rdf:resource="http://usefulinc.com/ns/doap#" />
	<rdfs:label xml:lang="en">mailing list</rdfs:label>
	<rdfs:label xml:lang="fr">liste de diffusion</rdfs:label>
	<rdfs:label xml:lang="es">lista de correo</rdfs:label>
	<rdfs:label xml:lang="de">Mailing Liste</rdfs:label>
	<rdfs:label xml:lang="cs">e–mailová diskuse</rdfs:label>
	<rdfs:label xml:lang="pt">lista de distribuição de e-mail</rdfs:label>
	<rdfs:label xml:lang="zh-CN">邮件列表</rdfs:label>
	<rdfs:comment xml:lang="en">Mailing list home page or email address.</rdfs:comment>
	<rdfs:comment xml:lang="fr">Page web de la liste de diffusion, ou adresse de courriel.</rdfs:comment>
	<rdfs:comment xml:lang="es">Página web de la lista de correo o dirección de correo.</rdfs:comment>
	<rdfs:comment xml:lang="de">Homepage der Mailing Liste oder E-Mail Adresse.</rdfs:comment>
	<rdfs:comment xml:lang="cs">Domovská stránka nebo e–mailová adresa e–mailové diskuse.</rdfs:comment>
	<rdfs:comment xml:lang="pt">Página web da lista de distribuição de e-mail ou dos endereços.</rdfs:comment>
	<rdfs:comment xml:lang="zh-CN">邮件列表的首页或Email地址。</rdfs:comment>
	<rdfs:domain rdf:resource="http://usefulinc.com/ns/doap#Project" />
	<rdfs:range rdf:resource="http://rdfs.org/sioc/types#MailingList" />
</rdf:Property>

<rdf:Property rdf:about="http://usefulinc.com/ns/doap#support-forum">
	<rdfs:isDefinedBy rdf:resource="http://usefulinc.com/ns/doap#" />
	<rdfs:label xml:lang="en">supporting forum</rdfs:label>
	<rdfs:label xml:lang="zh-CN">支持论坛</rdfs:label>
	<rdfs:comment xml:lang="en">A forum or community that supports this project.</rdfs:comment>
	<rdfs:comment xml:lang="zh-CN">支持这个项目的论坛或社区。</rdfs:comment>
	<rdfs:domain rdf:resource="http://usefulinc.com/ns/doap#Project" />
	<rdfs:range rdf:resource="http://rdfs.org/sioc/ns#Container" />
</rdf:Property>

<rdf:Property rdf:about="http://usefulinc.com/ns/doap#developer-forum">
	<rdfs:isDefinedBy rdf:resource="http://usefulinc.com/ns/doap#" />
	<rdfs:label xml:lang="en">developer forum</rdfs:label>
	<rdfs:label xml:lang="zh-CN">开发者论坛</rdfs:label>
	<rdfs:comment xml:lang="en">A forum or community for developers of this project.</rdfs:comment>
	<rdfs:comment xml:lang="zh-CN">项目开发者的论坛或社区。</rdfs:comment>
	<rdfs:domain rdf:resource="http://usefulinc.com/ns/doap#Project" />
	<rdfs:range rdf:resource="http://rdfs.org/sioc/ns#Container" />
</rdf:Property>


<rdf:Property rdf:about="http://usefulinc.com/ns/doap#category">
	<rdfs:isDefinedBy rdf:resource="http://usefulinc.com/ns/doap#" />
	<rdfs:label xml:lang="en">category</rdfs:label>
	<rdfs:label xml:lang="fr">catégorie</rdfs:label>
	<rdfs:label xml:lang="es">categoría</rdfs:label>
	<rdfs:label xml:lang="de">Kategorie</rdfs:label>
	<rdfs:label xml:lang="cs">kategorie</rdfs:label>
	<rdfs:label xml:lang="pt">categoria</rdfs:label>
	<rdfs:label xml:lang="zh-CN">分类</rdfs:label>
	<rdfs:comment xml:lang="en">A category of project.</rdfs:comment>
	<rdfs:comment xml:lang="fr">Une catégorie de projet.</rdfs:comment>
	<rdfs:comment xml:lang="es">Una categoría de proyecto.</rdfs:comment>
	<rdfs:comment xml:lang="de">Eine Kategorie eines Projektes.</rdfs:comment>
	<rdfs:comment xml:lang="cs">Kategorie projektu.</rdfs:comment>
	<rdfs:comment xml:lang="pt">Uma categoría de projeto.</rdfs:comment>
	<rdfs:comment xml:lang="zh-CN">项目的分类。</rdfs:comment>
	<rdfs:domain rdf:resource="http://usefulinc.com/ns/doap#Project" />
</rdf:Property>


<rdf:Property rdf:about="http://usefulinc.com/ns/doap#license">
	<rdfs:isDefinedBy rdf:resource="http://usefulinc.com/ns/doap#" />
	<rdfs:label xml:lang="en">license</rdfs:label>
	<rdfs:label xml:lang="fr">licence</rdfs:label>
	<rdfs:label xml:lang="es">licencia</rdfs:label>
	<rdfs:label xml:lang="de">Lizenz</rdfs:label>
	<rdfs:label xml:lang="cs">licence</rdfs:label>
	<rdfs:label xml:lang="pt">licença</rdfs:label>
	<rdfs:label xml:lang="zh-CN">版权</rdfs:label>
	<rdfs:comment xml:lang="en">The URI of an RDF description of the license the software is distributed under. E.g. a SPDX reference</rdfs:comment>
	<rdfs:comment xml:lang="fr">L'URI d'une description RDF de la licence sous laquelle le programme est distribué.</rdfs:comment>
	<rdfs:comment xml:lang="es">El URI de una descripción RDF de la licencia bajo la cuál se distribuye el software.</rdfs:comment>
	<rdfs:comment xml:lang="de">Die URI einer RDF-Beschreibung einer Lizenz unter der die Software herausgegeben wird. z.B. eine SPDX Referenz</rdfs:comment>
	<rdfs:comment xml:lang="cs">URI adresa RDF popisu licence, pod kterou je software distribuován.</rdfs:comment>
	<rdfs:comment xml:lang="pt">O URI de uma descrição RDF da licença do software sob a qual é distribuída. Ex.: referência SPDX</rdfs:comment>
	<rdfs:comment xml:lang="zh-CN">该软件分发使用的版权的RDF描述的URI，比如一个SPDX引用。</rdfs:comment>
</rdf:Property>

<rdf:Property rdf:about="http://usefulinc.com/ns/doap#repository">
	<rdfs:isDefinedBy rdf:resource="http://usefulinc.com/ns/doap#" />
	<rdfs:label xml:lang="en">repository</rdfs:label>
	<rdfs:label xml:lang="fr">dépôt</rdfs:label>
	<rdfs:label xml:lang="es">repositorio</rdfs:label>
	<rdfs:label xml:lang="de">Repository</rdfs:label>
	<rdfs:label xml:lang="cs">úložiště</rdfs:label>
	<rdfs:label xml:lang="pt">repositório</rdfs:label>
	<rdfs:label xml:lang="zh-CN">仓库</rdfs:label>
	<rdfs:comment xml:lang="en">Source code repository.</rdfs:comment>
	<rdfs:comment xml:lang="fr">Dépôt du code source.</rdfs:comment>
	<rdfs:comment xml:lang="es">Repositorio del código fuente.</rdfs:comment>
	<rdfs:comment xml:lang="de">Quellcode-Versionierungssystem.</rdfs:comment>
	<rdfs:comment xml:lang="cs">Úložiště zdrojových kódů.</rdfs:comment>
	<rdfs:comment xml:lang="pt">Repositório do código fonte.</rdfs:comment>
	<rdfs:comment xml:lang="zh-CN">源代码仓库。</rdfs:comment>
	<rdfs:domain rdf:resource="http://usefulinc.com/ns/doap#Project" />
	<rdfs:range rdf:resource="http://usefulinc.com/ns/doap#Repository" />
	<owl:inverseOf rdf:resource="http://usefulinc.com/ns/doap#repositoryOf" />
</rdf:Property>

<rdf:Property rdf:about="http://usefulinc.com/ns/doap#repositoryOf">
	<rdfs:isDefinedBy rdf:resource="http://usefulinc.com/ns/doap#" />
	<rdfs:label xml:lang="en">repository of</rdfs:label>
	<rdfs:label xml:lang="zh-CN">所属项目</rdfs:label>
	<rdfs:comment xml:lang="en">The project that uses a repository.</rdfs:comment>
	<rdfs:comment xml:lang="zh-CN">仓库的所属项目。</rdfs:comment>
	<rdfs:range rdf:resource="http://usefulinc.com/ns/doap#Project" />
	<rdfs:domain rdf:resource="http://usefulinc.com/ns/doap#Repository" />
	<owl:inverseOf rdf:resource="http://usefulinc.com/ns/doap#repository" />
</rdf:Property>

<rdf:Property rdf:about="http://usefulinc.com/ns/doap#anon-root">
	<rdfs:isDefinedBy rdf:resource="http://usefulinc.com/ns/doap#" />
	<rdfs:label xml:lang="en">anonymous root</rdfs:label>
	<rdfs:label xml:lang="fr">racine anonyme</rdfs:label>
	<rdfs:label xml:lang="es">raíz anónima</rdfs:label>
	<rdfs:label xml:lang="de">Anonymes Root</rdfs:label>
	<rdfs:label xml:lang="cs">anonymní kořen</rdfs:label>
	<rdfs:label xml:lang="pt">raíz anónima</rdfs:label>
	<rdfs:label xml:lang="zh-CN">匿名源</rdfs:label>
	<rdfs:comment xml:lang="en">Repository for anonymous access.</rdfs:comment>
	<rdfs:comment xml:lang="fr">Dépôt pour accès anonyme.</rdfs:comment>
	<rdfs:comment xml:lang="es">Repositorio para acceso anónimo.</rdfs:comment>
	<rdfs:comment xml:lang="de">Repository für anonymen Zugriff</rdfs:comment>
	<rdfs:comment xml:lang="cs">Úložiště pro anonymní přístup.</rdfs:comment>
	<rdfs:comment xml:lang="pt">Repositório para acesso anónimo.</rdfs:comment>
	<rdfs:comment xml:lang="zh-CN">用于匿名访问的仓库。</rdfs:comment>
	<rdfs:domain rdf:resource="http://usefulinc.com/ns/doap#Repository" />
	<rdfs:range rdf:resource="http://www.w3.org/2000/01/rdf-schema#Literal" />
</rdf:Property>

<rdf:Property rdf:about="http://usefulinc.com/ns/doap#browse">
	<rdfs:isDefinedBy rdf:resource="http://usefulinc.com/ns/doap#" />
	<rdfs:label xml:lang="en">browse</rdfs:label>
	<rdfs:label xml:lang="fr">visualiser</rdfs:label>
	<rdfs:label xml:lang="es">navegar</rdfs:label>
	<rdfs:label xml:lang="de">browse</rdfs:label>
	<rdfs:label xml:lang="cs">prohlížeč</rdfs:label>
	<rdfs:label xml:lang="pt">navegar</rdfs:label>
	<rdfs:label xml:lang="zh-CN">浏览</rdfs:label>
	<rdfs:comment xml:lang="en">Web browser interface to repository.</rdfs:comment>
	<rdfs:comment xml:lang="fr">Interface web au dépôt.</rdfs:comment>
	<rdfs:comment xml:lang="es">Interface web del repositorio.</rdfs:comment>
	<rdfs:comment xml:lang="de">Web-Browser Interface für das Repository.</rdfs:comment>
	<rdfs:comment xml:lang="cs">Webové rozhraní pro prohlížení úložiště.</rdfs:comment>
	<rdfs:comment xml:lang="pt">Interface web do repositório.</rdfs:comment>
	<rdfs:comment xml:lang="zh-CN">仓库的网络浏览器界面。</rdfs:comment>
	<rdfs:domain rdf:resource="http://usefulinc.com/ns/doap#Repository" />
</rdf:Property>

<rdf:Property rdf:about="http://usefulinc.com/ns/doap#module">
	<rdfs:isDefinedBy rdf:resource="http://usefulinc.com/ns/doap#" />
	<rdfs:label xml:lang="en">module</rdfs:label>
	<rdfs:label xml:lang="fr">module</rdfs:label>
	<rdfs:label xml:lang="es">módulo</rdfs:label>
	<rdfs:label xml:lang="de">Modul</rdfs:label>
	<rdfs:label xml:lang="cs">modul</rdfs:label>
	<rdfs:label xml:lang="pt">módulo</rdfs:label>
	<rdfs:label xml:lang="zh-CN">模块</rdfs:label>
	<rdfs:comment xml:lang="en">Module name of a Subversion, CVS, BitKeeper or Arch repository.</rdfs:comment>
	<rdfs:comment xml:lang="fr">Nom du module d'un dépôt Subversion, CVS, BitKeeper ou Arch.</rdfs:comment>
	<rdfs:comment xml:lang="es">Nombre del módulo de un repositorio Subversion, CVS, BitKeeper o Arch.</rdfs:comment>
	<rdfs:comment xml:lang="de">Modul-Name eines Subversion, CVS, BitKeeper oder Arch Repositorys.</rdfs:comment>
	<rdfs:comment xml:lang="cs">Jméno modulu v CVS, BitKeeper nebo Arch úložišti.</rdfs:comment>
	<rdfs:comment xml:lang="pt">Nome do módulo de um repositório Subversion, CVS, BitKeeper ou Arch.</rdfs:comment>
	<rdfs:comment xml:lang="zh-CN">Subversion、CVS、BitKeeper或Arch仓库的模块名称。</rdfs:comment>
	<!-- doesn't apply to subversion repositories -->
	<rdfs:domain>
	  <owl:Class>
		<owl:unionOf rdf:parseType="Collection">
		  <owl:Class rdf:about="http://usefulinc.com/ns/doap#CVSRepository" />
		  <owl:Class rdf:about="http://usefulinc.com/ns/doap#ArchRepository" />
		  <owl:Class rdf:about="http://usefulinc.com/ns/doap#BKRepository" />
		</owl:unionOf>
	  </owl:Class>
	</rdfs:domain>
</rdf:Property>

<rdf:Property rdf:about="http://usefulinc.com/ns/doap#location">
	<rdfs:isDefinedBy rdf:resource="http://usefulinc.com/ns/doap#" />
	<rdfs:label xml:lang="en">repository location</rdfs:label>
	<rdfs:label xml:lang="fr">emplacement du dépôt</rdfs:label>
	<rdfs:label xml:lang="es">lugar del respositorio</rdfs:label>
	<rdfs:label xml:lang="de">Repository Lokation</rdfs:label>
	<rdfs:label xml:lang="cs">umístění úložiště</rdfs:label>
	<rdfs:label xml:lang="pt">localização do respositório</rdfs:label>
	<rdfs:label xml:lang="zh-CN">仓库地址</rdfs:label>
	<rdfs:comment xml:lang="en">Location of a repository.</rdfs:comment>
	<rdfs:comment xml:lang="fr">Emplacement d'un dépôt.</rdfs:comment>
	<rdfs:comment xml:lang="es">lugar de un repositorio.</rdfs:comment>
	<rdfs:comment xml:lang="de">Lokation eines Repositorys.</rdfs:comment>
	<rdfs:comment xml:lang="cs">Umístění úložiště.</rdfs:comment>
	<rdfs:comment xml:lang="pt">Localização de um repositório.</rdfs:comment>
	<rdfs:comment xml:lang="zh-CN">仓库的地址。</rdfs:comment>
	<rdfs:domain rdf:resource="http://usefulinc.com/ns/doap#Repository" />
</rdf:Property>

<rdf:Property rdf:about="http://usefulinc.com/ns/doap#download-page">
	<rdfs:isDefinedBy rdf:resource="http://usefulinc.com/ns/doap#" />
	<rdfs:label xml:lang="en">download page</rdfs:label>
	<rdfs:label xml:lang="fr">page de téléchargement</rdfs:label>
	<rdfs:label xml:lang="es">página de descarga</rdfs:label>
	<rdfs:label xml:lang="de">Seite zum Herunterladen</rdfs:label>
	<rdfs:label xml:lang="cs">stránka pro stažení</rdfs:label>
	<rdfs:label xml:lang="pt">página para download</rdfs:label>
	<rdfs:label xml:lang="zh-CN">下载页面</rdfs:label>
	<rdfs:comment xml:lang="en">Web page from which the project software can be downloaded.</rdfs:comment>
	<rdfs:comment xml:lang="fr">Page web à partir de laquelle on peut télécharger le programme.</rdfs:comment>
	<rdfs:comment xml:lang="es">Página web de la cuál se puede bajar el software.</rdfs:comment>
	<rdfs:comment xml:lang="de">Web-Seite von der die Projekt-Software heruntergeladen werden kann.</rdfs:comment>
	<rdfs:comment xml:lang="cs">Webová stránka, na které lze stáhnout projektový software.</rdfs:comment>
	<rdfs:comment xml:lang="pt">Página web da qual o projeto de software pode ser descarregado.</rdfs:comment>
	<rdfs:comment xml:lang="zh-CN">可以下载该项目软件的网页。</rdfs:comment>
	<rdfs:domain rdf:resource="http://usefulinc.com/ns/doap#Project" />
</rdf:Property>

<rdf:Property rdf:about="http://usefulinc.com/ns/doap#download-mirror">
	<rdfs:isDefinedBy rdf:resource="http://usefulinc.com/ns/doap#" />
	<rdfs:label xml:lang="en">download mirror</rdfs:label>
	<rdfs:label xml:lang="fr">miroir pour le téléchargement</rdfs:label>
	<rdfs:label xml:lang="es">mirror de descarga</rdfs:label>
	<rdfs:label xml:lang="de">Spiegel der Seite zum Herunterladen</rdfs:label>
	<rdfs:label xml:lang="cs">zrcadlo stránky pro stažení</rdfs:label>
	<rdfs:label xml:lang="pt">mirror para download</rdfs:label>
	<rdfs:label xml:lang="zh-CN">下载镜像</rdfs:label>
	<rdfs:comment xml:lang="en">Mirror of software download web page.</rdfs:comment>
	<rdfs:comment xml:lang="fr">Miroir de la page de téléchargement du programme.</rdfs:comment>
	<rdfs:comment xml:lang="es">Mirror de la página web de descarga.</rdfs:comment>
	<rdfs:comment xml:lang="de">Spiegel der Seite von die Projekt-Software heruntergeladen werden kann.</rdfs:comment>
	<rdfs:comment xml:lang="cs">Zrcadlo stránky pro stažení softwaru.</rdfs:comment>
	<rdfs:comment xml:lang="pt">Mirror da página web para fazer download.</rdfs:comment>
	<rdfs:comment xml:lang="zh-CN">软件下载网页的镜像。</rdfs:comment>
	<rdfs:domain rdf:resource="http://usefulinc.com/ns/doap#Project" />
</rdf:Property>

<rdf:Property rdf:about="http://usefulinc.com/ns/doap#revision">
	<rdfs:isDefinedBy rdf:resource="http://usefulinc.com/ns/doap#" />
	<rdfs:label xml:lang="en">revision</rdfs:label>
	<rdfs:label xml:lang="fr">révision</rdfs:label>
	<rdfs:label xml:lang="es">versión</rdfs:label>
	<rdfs:label xml:lang="de">Version</rdfs:label>
	<rdfs:label xml:lang="cs">verze</rdfs:label>
	<rdfs:label xml:lang="pt">revisão</rdfs:label>
	<rdfs:label xml:lang="zh-CN">修订标识</rdfs:label>
	<rdfs:comment xml:lang="en">Revision identifier of a software release.</rdfs:comment>
	<rdfs:comment xml:lang="fr">Identifiant de révision d'une release du programme.</rdfs:comment>
	<rdfs:comment xml:lang="es">Indentificador de la versión de un release de software.</rdfs:comment>
	<rdfs:comment xml:lang="de">Versionsidentifikator eines Software-Releases.</rdfs:comment>
	<rdfs:comment xml:lang="cs">Identifikátor zpřístupněné revize softwaru.</rdfs:comment>
	<rdfs:comment xml:lang="pt">Identificador do lançamento da revisão do software.</rdfs:comment>
	<rdfs:comment xml:lang="zh-CN">软件发行的修订标识。</rdfs:comment>
	<rdfs:domain rdf:resource="http://usefulinc.com/ns/doap#Version" />
	<rdfs:range rdf:resource="http://www.w3.org/2000/01/rdf-schema#Literal" />
</rdf:Property>

<rdf:Property rdf:about="http://usefulinc.com/ns/doap#file-release">
	<rdfs:isDefinedBy rdf:resource="http://usefulinc.com/ns/doap#" />
	<rdfs:label xml:lang="en">file-release</rdfs:label>
	<rdfs:label xml:lang="cs">soubor revize</rdfs:label>
	<rdfs:label xml:lang="pt">publicação do ficheiro</rdfs:label>
	<rdfs:label xml:lang="zh-CN">发行文件</rdfs:label>
	<rdfs:comment xml:lang="en">URI of download associated with this release.</rdfs:comment>
	<rdfs:comment xml:lang="cs">URI adresa stažení asociované s revizí.</rdfs:comment>
	<rdfs:comment xml:lang="pt">URI para download associado com a publicação.</rdfs:comment>
	<rdfs:comment xml:lang="zh-CN">与该发行关联的下载URI。</rdfs:comment>
	<rdfs:domain rdf:resource="http://usefulinc.com/ns/doap#Version" />
</rdf:Property>

<rdf:Property rdf:about="http://usefulinc.com/ns/doap#wiki">
	<rdfs:isDefinedBy rdf:resource="http://usefulinc.com/ns/doap#" />
	<rdfs:label xml:lang="en">wiki</rdfs:label>
	<rdfs:label xml:lang="fr">wiki</rdfs:label>
	<rdfs:label xml:lang="es">wiki</rdfs:label>
	<rdfs:label xml:lang="de">Wiki</rdfs:label>
	<rdfs:label xml:lang="cs">wiki</rdfs:label>
	<rdfs:label xml:lang="pt">wiki</rdfs:label>
	<rdfs:label xml:lang="zh-CN">wiki</rdfs:label>
	<rdfs:comment xml:lang="en">URL of Wiki for collaborative discussion of project.</rdfs:comment>
	<rdfs:comment xml:lang="fr">L'URL du Wiki pour la discussion collaborative sur le projet.</rdfs:comment>
	<rdfs:comment xml:lang="es">URL del Wiki para discusión colaborativa del proyecto.</rdfs:comment>
	<rdfs:comment xml:lang="de">Wiki-URL für die kollaborative Dikussion eines Projektes.</rdfs:comment>
	<rdfs:comment xml:lang="cs">URL adresa wiki projektu pro společné diskuse.</rdfs:comment>
	<rdfs:comment xml:lang="pt">URL da Wiki para discussão em grupo do projeto.</rdfs:comment>
	<rdfs:comment xml:lang="zh-CN">用于项目协作讨论的Wiki的URL。</rdfs:comment>
	<rdfs:domain rdf:resource="http://usefulinc.com/ns/doap#Project" />
    <rdfs:range rdf:resource="http://rdfs.org/sioc/types#Wiki" />
</rdf:Property>

<rdf:Property rdf:about="http://usefulinc.com/ns/doap#bug-database">
	<rdfs:isDefinedBy rdf:resource="http://usefulinc.com/ns/doap#" />
	<rdfs:label xml:lang="en">bug database</rdfs:label>
	<rdfs:label xml:lang="fr">suivi des bugs</rdfs:label>
	<rdfs:label xml:lang="es">base de datos de bugs</rdfs:label>
	<rdfs:label xml:lang="de">Fehlerdatenbank</rdfs:label>
	<rdfs:label xml:lang="cs">databáze chyb</rdfs:label>
	<rdfs:label xml:lang="pt">base de dados de bugs</rdfs:label>
	<rdfs:label xml:lang="zh-CN">漏洞数据库</rdfs:label>
	<rdfs:comment xml:lang="en">Bug tracker for a project.</rdfs:comment>
	<rdfs:comment xml:lang="fr">Suivi des bugs pour un projet.</rdfs:comment>
	<rdfs:comment xml:lang="es">Bug tracker para un proyecto.</rdfs:comment>
	<rdfs:comment xml:lang="de">Fehlerdatenbank eines Projektes.</rdfs:comment>
	<rdfs:comment xml:lang="cs">Správa chyb projektu.</rdfs:comment>
	<rdfs:comment xml:lang="pt">Bug tracker para um projeto.</rdfs:comment>
	<rdfs:comment xml:lang="zh-CN">项目的漏洞跟踪程序。</rdfs:comment>
	<rdfs:domain rdf:resource="http://usefulinc.com/ns/doap#Project" />
</rdf:Property>

<rdf:Property rdf:about="http://usefulinc.com/ns/doap#documentation">
	<rdfs:isDefinedBy rdf:resource="http://usefulinc.com/ns/doap#" />
	<rdfs:label xml:lang="en">documentation</rdfs:label>
	<rdfs:label xml:lang="fr">aide</rdfs:label>
	<rdfs:comment xml:lang="en">Documentation of the project.</rdfs:comment>
	<rdfs:comment xml:lang="fr">Aide pour l’utilisation de ce projet.</rdfs:comment>
	<rdfs:domain rdf:resource="http://usefulinc.com/ns/doap#Project" />
</rdf:Property>

<rdf:Property rdf:about="http://usefulinc.com/ns/doap#screenshots">
	<rdfs:isDefinedBy rdf:resource="http://usefulinc.com/ns/doap#" />
	<rdfs:label xml:lang="en">screenshots</rdfs:label>
	<rdfs:label xml:lang="fr">captures d'écran</rdfs:label>
	<rdfs:label xml:lang="es">capturas de pantalla</rdfs:label>
	<rdfs:label xml:lang="de">Screenshots</rdfs:label>
	<rdfs:label xml:lang="cs">snímek obrazovky</rdfs:label>
	<rdfs:label xml:lang="pt">capturas de ecrãs</rdfs:label>
	<rdfs:label xml:lang="zh-CN">截屏</rdfs:label>
	<rdfs:comment xml:lang="en">Web page with screenshots of project.</rdfs:comment>
	<rdfs:comment xml:lang="fr">Page web avec des captures d'écran du projet.</rdfs:comment>
	<rdfs:comment xml:lang="es">Página web con capturas de pantalla del proyecto.</rdfs:comment>
	<rdfs:comment xml:lang="de">Web-Seite mit Screenshots eines Projektes.</rdfs:comment>
	<rdfs:comment xml:lang="cs">Webová stránka projektu se snímky obrazovky.</rdfs:comment>
	<rdfs:comment xml:lang="pt">Página web com as capturas de ecrãn do projeto.</rdfs:comment>
	<rdfs:comment xml:lang="zh-CN">项目截屏的网页。</rdfs:comment>
	<rdfs:domain rdf:resource="http://usefulinc.com/ns/doap#Project" />
</rdf:Property>

<rdf:Property rdf:about="http://usefulinc.com/ns/doap#maintainer">
	<rdfs:isDefinedBy rdf:resource="http://usefulinc.com/ns/doap#" />
	<rdfs:label xml:lang="en">maintainer</rdfs:label>
	<rdfs:label xml:lang="fr">développeur principal</rdfs:label>
	<rdfs:label xml:lang="es">desarrollador principal</rdfs:label>
	<rdfs:label xml:lang="de">Projektverantwortlicher</rdfs:label>
	<rdfs:label xml:lang="cs">správce</rdfs:label>
	<rdfs:label xml:lang="pt">programador principal</rdfs:label>
	<rdfs:label xml:lang="zh-CN">维护者</rdfs:label>
	<rdfs:comment xml:lang="en">Maintainer of a project, a project leader.</rdfs:comment>
	<rdfs:comment xml:lang="fr">Développeur principal d'un projet, un meneur du projet.</rdfs:comment>
	<rdfs:comment xml:lang="es">Desarrollador principal de un proyecto, un líder de proyecto.</rdfs:comment>
	<rdfs:comment xml:lang="de">Hauptentwickler eines Projektes, der Projektleiter</rdfs:comment>
	<rdfs:comment xml:lang="cs">Správce projektu, vedoucí projektu.</rdfs:comment>
	<rdfs:comment xml:lang="pt">Programador principal de um projeto, um líder de projeto.</rdfs:comment>
	<rdfs:comment xml:lang="zh-CN">项目的维护者，项目的领导者。</rdfs:comment>
	<rdfs:domain rdf:resource="http://usefulinc.com/ns/doap#Project" />
	<rdfs:range rdf:resource="http://xmlns.com/foaf/0.1/Person" />
</rdf:Property>

<rdf:Property rdf:about="http://usefulinc.com/ns/doap#developer">
	<rdfs:isDefinedBy rdf:resource="http://usefulinc.com/ns/doap#" />
	<rdfs:label xml:lang="en">developer</rdfs:label>
	<rdfs:label xml:lang="fr">développeur</rdfs:label>
	<rdfs:label xml:lang="es">desarrollador</rdfs:label>
	<rdfs:label xml:lang="de">Entwickler</rdfs:label>
	<rdfs:label xml:lang="cs">vývojář</rdfs:label>
	<rdfs:label xml:lang="pt">programador</rdfs:label>
	<rdfs:label xml:lang="zh-CN">开发者</rdfs:label>
	<rdfs:comment xml:lang="en">Developer of software for the project.</rdfs:comment>
	<rdfs:comment xml:lang="fr">Développeur pour le projet.</rdfs:comment>
	<rdfs:comment xml:lang="es">Desarrollador de software para el proyecto.</rdfs:comment>
	<rdfs:comment xml:lang="de">Software-Entwickler für das Projekt.</rdfs:comment>
	<rdfs:comment xml:lang="cs">Vývojář softwaru projektu.</rdfs:comment>
	<rdfs:comment xml:lang="pt">Programador de software para o projeto.</rdfs:comment>
	<rdfs:comment xml:lang="zh-CN">项目的软件开发者。</rdfs:comment>
	<rdfs:domain rdf:resource="http://usefulinc.com/ns/doap#Project" />
	<rdfs:range rdf:resource="http://xmlns.com/foaf/0.1/Person" />
</rdf:Property>

<rdf:Property rdf:about="http://usefulinc.com/ns/doap#security-contact">
	<rdfs:isDefinedBy rdf:resource="http://usefulinc.com/ns/doap#" />
	<rdfs:label xml:lang="en">security contact</rdfs:label>
	<rdfs:comment xml:lang="en">The Agent that should be contacted
	if security issues are found with the project.</rdfs:comment>
	<rdfs:domain rdf:resource="http://usefulinc.com/ns/doap#Project" />
	<rdfs:range rdf:resource="http://xmlns.com/foaf/0.1/Agent" />
</rdf:Property>

<rdf:Property rdf:about="http://usefulinc.com/ns/doap#documenter">
	<rdfs:isDefinedBy rdf:resource="http://usefulinc.com/ns/doap#" />
	<rdfs:label xml:lang="en">documenter</rdfs:label>
	<rdfs:label xml:lang="fr">rédacteur de l'aide</rdfs:label>
	<rdfs:label xml:lang="es">escritor de ayuda</rdfs:label>
	<rdfs:label xml:lang="de">Dokumentator</rdfs:label>
	<rdfs:label xml:lang="cs">dokumentarista</rdfs:label>
	<rdfs:label xml:lang="pt">documentador</rdfs:label>
	<rdfs:label xml:lang="zh-CN">文档编辑</rdfs:label>
	<rdfs:comment xml:lang="en">Contributor of documentation to the project.</rdfs:comment>
	<rdfs:comment xml:lang="fr">Collaborateur à la documentation du projet.</rdfs:comment>
	<rdfs:comment xml:lang="es">Proveedor de documentación para el proyecto.</rdfs:comment>
	<rdfs:comment xml:lang="de">Mitarbeiter an der Dokumentation des Projektes.</rdfs:comment>
	<rdfs:comment xml:lang="cs">Spoluautor dokumentace projektu.</rdfs:comment>
	<rdfs:comment xml:lang="pt">Contribuidor para a documentação do projeto.</rdfs:comment>
	<rdfs:comment xml:lang="zh-CN">项目文档的贡献者。</rdfs:comment>
	<rdfs:domain rdf:resource="http://usefulinc.com/ns/doap#Project" />
	<rdfs:range rdf:resource="http://xmlns.com/foaf/0.1/Person" />
</rdf:Property>

<rdf:Property rdf:about="http://usefulinc.com/ns/doap#translator">
	<rdfs:isDefinedBy rdf:resource="http://usefulinc.com/ns/doap#" />
	<rdfs:label xml:lang="en">translator</rdfs:label>
	<rdfs:label xml:lang="fr">traducteur</rdfs:label>
	<rdfs:label xml:lang="es">traductor</rdfs:label>
	<rdfs:label xml:lang="de">Übersetzer</rdfs:label>
	<rdfs:label xml:lang="cs">překladatel</rdfs:label>
	<rdfs:label xml:lang="pt">tradutor</rdfs:label>
	<rdfs:label xml:lang="zh-CN">翻译者</rdfs:label>
	<rdfs:comment xml:lang="en">Contributor of translations to the project.</rdfs:comment>
	<rdfs:comment xml:lang="fr">Collaborateur à la traduction du projet.</rdfs:comment>
	<rdfs:comment xml:lang="es">Proveedor de traducciones al proyecto.</rdfs:comment>
	<rdfs:comment xml:lang="de">Mitarbeiter an den Übersetzungen des Projektes.</rdfs:comment>
	<rdfs:comment xml:lang="cs">Spoluautor překladu projektu.</rdfs:comment>
	<rdfs:comment xml:lang="pt">Contribuidor das traduções para o projeto.</rdfs:comment>
	<rdfs:comment xml:lang="zh-CN">项目翻译的贡献者。</rdfs:comment>
	<rdfs:domain rdf:resource="http://usefulinc.com/ns/doap#Project" />
	<rdfs:range rdf:resource="http://xmlns.com/foaf/0.1/Person" />
</rdf:Property>

<rdf:Property rdf:about="http://usefulinc.com/ns/doap#tester">
	<rdfs:isDefinedBy rdf:resource="http://usefulinc.com/ns/doap#" />
	<rdfs:label xml:lang="en">tester</rdfs:label>
	<rdfs:label xml:lang="fr">testeur</rdfs:label>
	<rdfs:label xml:lang="es">tester</rdfs:label>
	<rdfs:label xml:lang="de">Tester</rdfs:label>
	<rdfs:label xml:lang="cs">tester</rdfs:label>
	<rdfs:label xml:lang="pt">controlador</rdfs:label>
	<rdfs:label xml:lang="zh-CN">测试者</rdfs:label>
	<rdfs:comment xml:lang="en">A tester or other quality control contributor.</rdfs:comment>
	<rdfs:comment xml:lang="fr">Un testeur ou un collaborateur au contrôle qualité.</rdfs:comment>
	<rdfs:comment xml:lang="es">Un tester u otro proveedor de control de calidad.</rdfs:comment>
	<rdfs:comment xml:lang="de">Ein Tester oder anderer Mitarbeiter der Qualitätskontrolle.</rdfs:comment>
	<rdfs:comment xml:lang="cs">Tester nebo jiný spoluautor kontrolující kvalitu.</rdfs:comment>
	<rdfs:comment xml:lang="pt">Um controlador ou outro contribuidor para o controlo de qualidade.</rdfs:comment>
	<rdfs:comment xml:lang="zh-CN">测试人或其他质量控制的贡献者。</rdfs:comment>
	<rdfs:domain rdf:resource="http://usefulinc.com/ns/doap#Project" />
	<rdfs:range rdf:resource="http://xmlns.com/foaf/0.1/Person" />
</rdf:Property>

<rdf:Property rdf:about="http://usefulinc.com/ns/doap#helper">
	<rdfs:isDefinedBy rdf:resource="http://usefulinc.com/ns/doap#" />
	<rdfs:label xml:lang="en">helper</rdfs:label>
	<rdfs:label xml:lang="fr">collaborateur</rdfs:label>
	<rdfs:label xml:lang="es">colaborador</rdfs:label>
	<rdfs:label xml:lang="de">Helfer</rdfs:label>
	<rdfs:label xml:lang="cs">spoluautor</rdfs:label>
	<rdfs:label xml:lang="pt">colaborador</rdfs:label>
	<rdfs:label xml:lang="zh-CN">帮助者</rdfs:label>
	<rdfs:comment xml:lang="en">Project contributor.</rdfs:comment>
	<rdfs:comment xml:lang="fr">Collaborateur au projet.</rdfs:comment>
	<rdfs:comment xml:lang="es">Colaborador del proyecto.</rdfs:comment>
	<rdfs:comment xml:lang="de">Projekt-Mitarbeiter.</rdfs:comment>
	<rdfs:comment xml:lang="cs">Spoluautor projektu.</rdfs:comment>
	<rdfs:comment xml:lang="pt">Ajudante ou colaborador do projeto.</rdfs:comment>
	<rdfs:comment xml:lang="zh-CN">项目的贡献者。</rdfs:comment>
	<rdfs:domain rdf:resource="http://usefulinc.com/ns/doap#Project" />
	<rdfs:range rdf:resource="http://xmlns.com/foaf/0.1/Person" />
</rdf:Property>

<rdf:Property rdf:about="http://usefulinc.com/ns/doap#programming-language">
	<rdfs:isDefinedBy rdf:resource="http://usefulinc.com/ns/doap#" />
	<rdfs:label xml:lang="en">programming language</rdfs:label>
	<rdfs:label xml:lang="fr">langage de programmation</rdfs:label>
	<rdfs:label xml:lang="es">lenguaje de programación</rdfs:label>
	<rdfs:label xml:lang="de">Programmiersprache</rdfs:label>
	<rdfs:label xml:lang="cs">programovací jazyk</rdfs:label>
	<rdfs:label xml:lang="pt">linguagem de programação</rdfs:label>
	<rdfs:label xml:lang="zh-CN">开发语言</rdfs:label>
	<rdfs:comment xml:lang="en">Programming language a project is implemented in or intended for use with.</rdfs:comment>
	<rdfs:comment xml:lang="fr">Langage de programmation avec lequel un projet est implémenté,
		ou avec lequel il est prévu de l'utiliser.</rdfs:comment>
	<rdfs:comment xml:lang="es">Lenguaje de programación en el que un proyecto es implementado o con el cuál pretende usarse.</rdfs:comment>
	<rdfs:comment xml:lang="de">Programmiersprache in der ein Projekt implementiert ist oder intendiert wird zu benutzen.</rdfs:comment>
	<rdfs:comment xml:lang="cs">Programovací jazyk, ve kterém je projekt implementován nebo pro který je zamýšlen k použití.</rdfs:comment>
	<rdfs:comment xml:lang="pt">Linguagem de programação que o projeto usa ou é para ser utilizada.</rdfs:comment>
	<rdfs:comment xml:lang="zh-CN">项目实现或准备在项目中使用的开发语言。</rdfs:comment>
	<rdfs:domain rdf:resource="http://usefulinc.com/ns/doap#Project" />
	<rdfs:range rdf:resource="http://www.w3.org/2000/01/rdf-schema#Literal" />
</rdf:Property>

<rdf:Property rdf:about="http://usefulinc.com/ns/doap#os">
	<rdfs:isDefinedBy rdf:resource="http://usefulinc.com/ns/doap#" />
	<rdfs:label xml:lang="en">operating system</rdfs:label>
	<rdfs:label xml:lang="fr">système d'exploitation</rdfs:label>
	<rdfs:label xml:lang="es">sistema operativo</rdfs:label>
	<rdfs:label xml:lang="de">Betriebssystem</rdfs:label>
	<rdfs:label xml:lang="cs">operační systém</rdfs:label>
	<rdfs:label xml:lang="pt">sistema operativo</rdfs:label>
	<rdfs:label xml:lang="zh-CN">操作系统</rdfs:label>
	<rdfs:comment xml:lang="en">Operating system that a project is limited to.  Omit this property if the project is not OS-specific.</rdfs:comment>
	<rdfs:comment xml:lang="fr">Système d'exploitation auquel est limité le projet. Omettez cette propriété si le
		projet n'est pas limité à un système d'exploitation.</rdfs:comment>
	<rdfs:comment xml:lang="es">Sistema opertivo al cuál está limitado el proyecto.  Omita esta propiedad si el proyecto no es específico
		de un sistema opertaivo en particular.</rdfs:comment>
	<rdfs:comment xml:lang="de">Betriebssystem auf dem das Projekt eingesetzt werden kann. Diese Eigenschaft kann ausgelassen werden, wenn das Projekt nicht BS-spezifisch ist.</rdfs:comment>
	<rdfs:comment xml:lang="cs">Operační systém, na jehož použití je projekt limitován. Vynechejte tuto vlastnost, pokud je projekt nezávislý na operačním systému.</rdfs:comment>
	<rdfs:comment xml:lang="en">Sistema operativo a que o projeto está limitado. Omita esta propriedade se o projeto não é condicionado pelo SO usado.</rdfs:comment>
	<rdfs:comment xml:lang="zh-CN">项目受限的操作系统。如果项目是无关操作系统的，忽略该属性。</rdfs:comment>
	<rdfs:domain rdf:resource="http://usefulinc.com/ns/doap#Project" />
	<rdfs:domain rdf:resource="http://usefulinc.com/ns/doap#Version" />
	<rdfs:range rdf:resource="http://www.w3.org/2000/01/rdf-schema#Literal" />
</rdf:Property>

<rdf:Property rdf:about="http://usefulinc.com/ns/doap#implements">
	<rdfs:isDefinedBy rdf:resource="http://usefulinc.com/ns/doap#" />
	<rdfs:label xml:lang="en">Implements specification</rdfs:label>
	<rdfs:label xml:lang="pt">Especificações para implementação</rdfs:label>
	<rdfs:label xml:lang="zh-CN">实现规范</rdfs:label>
	<rdfs:comment xml:lang="en">A specification that a project implements. Could be a standard, API or legally defined level of conformance.</rdfs:comment>
	<rdfs:comment xml:lang="pt">Uma especificação que um projeto implementa. Pode ser uma padrão, API ou um nível de conformidade definida legalmente.</rdfs:comment>
	<rdfs:comment xml:lang="zh-CN">项目实现的规范。可以是标准、API或者法定的一致性级别。</rdfs:comment>
	<rdfs:domain rdf:resource="http://usefulinc.com/ns/doap#Project" />
	<rdfs:range rdf:resource="http://usefulinc.com/ns/doap#Specification" />
</rdf:Property>

<rdf:Property rdf:about="http://usefulinc.com/ns/doap#service-endpoint">
	<rdfs:isDefinedBy rdf:resource="http://usefulinc.com/ns/doap#" />
	<rdfs:label xml:lang="en">service endpoint</rdfs:label>
	<rdfs:label xml:lang="zh-CN">服务端点</rdfs:label>
	<rdfs:comment xml:lang="en">The URI of a web service endpoint where software as a service may be accessed</rdfs:comment>
	<rdfs:comment xml:lang="zh-CN">软件可以作为服务访问的网络服务端点URI。</rdfs:comment>
	<rdfs:domain rdf:resource="http://usefulinc.com/ns/doap#Project" />
	<rdfs:range rdf:resource="http://www.w3.org/2000/01/rdf-schema#Resource" />
</rdf:Property>

<rdf:Property rdf:about="http://usefulinc.com/ns/doap#language">
	<rdfs:isDefinedBy rdf:resource="http://usefulinc.com/ns/doap#" />
	<rdfs:label xml:lang="en">language</rdfs:label>
	<rdfs:label xml:lang="pt">idioma</rdfs:label>
	<rdfs:label xml:lang="zh-CN">语言</rdfs:label>
	<rdfs:comment xml:lang="en">ISO language code a project has been translated into</rdfs:comment>
	<rdfs:comment xml:lang="pt">Código de idioma ISO do projeto para o qual foi traduzido</rdfs:comment>
	<rdfs:comment xml:lang="zh-CN">项目支持的ISO语言代码。</rdfs:comment>
	<rdfs:domain rdf:resource="http://usefulinc.com/ns/doap#Project" />
	<rdfs:range rdf:resource="http://www.w3.org/2000/01/rdf-schema#Literal" />
</rdf:Property>

<rdf:Property rdf:about="http://usefulinc.com/ns/doap#vendor">
	<rdfs:isDefinedBy rdf:resource="http://usefulinc.com/ns/doap#" />
	<rdfs:label xml:lang="en">vendor</rdfs:label>
	<rdfs:label xml:lang="zh-CN">卖方</rdfs:label>
	<rdfs:comment xml:lang="en">Vendor organization: commercial, free or otherwise</rdfs:comment>
	<rdfs:comment xml:lang="zh-CN">售卖组织：商业的、免费的或其他。</rdfs:comment>
	<rdfs:domain rdf:resource="http://usefulinc.com/ns/doap#Project" />
	<rdfs:range rdf:resource="http://xmlns.com/foaf/0.1/Organization" />
</rdf:Property>

<rdf:Property rdf:about="http://usefulinc.com/ns/doap#platform">
	<rdfs:isDefinedBy rdf:resource="http://usefulinc.com/ns/doap#" />
	<rdfs:label xml:lang="en">platform</rdfs:label>
	<rdfs:label xml:lang="pt">plataforma</rdfs:label>
	<rdfs:label xml:lang="zh-CN">平台</rdfs:label>
	<rdfs:comment xml:lang="en">Indicator of software platform (non-OS specific), e.g. Java, Firefox, ECMA CLR</rdfs:comment>
	<rdfs:comment xml:lang="pt">Indicador da plataforma do software (não específico a nenhum SO), ex.: Java, Firefox, ECMA CLR</rdfs:comment>
	<rdfs:comment xml:lang="zh-CN">软件平台标识（无关操作系统），比如Java、Firefox、ECMA CLR。</rdfs:comment>
	<rdfs:domain rdf:resource="http://usefulinc.com/ns/doap#Project" />
	<rdfs:domain rdf:resource="http://usefulinc.com/ns/doap#Version" />
	<rdfs:range rdf:resource="http://www.w3.org/2000/01/rdf-schema#Literal" />
</rdf:Property>

<rdf:Property rdf:about="http://usefulinc.com/ns/doap#audience">
	<rdfs:isDefinedBy rdf:resource="http://usefulinc.com/ns/doap#" />
	<rdfs:label xml:lang="en">audience</rdfs:label>
	<rdfs:label xml:lang="pt">audiência</rdfs:label>
	<rdfs:label xml:lang="zh-CN">受众</rdfs:label>
	<rdfs:comment xml:lang="en">Description of target user base</rdfs:comment>
	<rdfs:comment xml:lang="pt">Descrição do utilizador base alvo</rdfs:comment>
	<rdfs:comment xml:lang="zh-CN">有关目标用户群的描述。</rdfs:comment>
	<rdfs:domain rdf:resource="http://usefulinc.com/ns/doap#Project" />
	<rdfs:range rdf:resource="http://www.w3.org/2000/01/rdf-schema#Literal" />
</rdf:Property>

<rdf:Property rdf:about="http://usefulinc.com/ns/doap#blog">
	<rdfs:isDefinedBy rdf:resource="http://usefulinc.com/ns/doap#" />
	<rdfs:label xml:lang="en">blog</rdfs:label>
	<rdfs:label xml:lang="pt">blog</rdfs:label>
	<rdfs:label xml:lang="zh-CN">博客</rdfs:label>
	<rdfs:comment xml:lang="en">URI of a blog related to a project</rdfs:comment>
	<rdfs:comment xml:lang="pt">URI de um blog relacionado com um projeto</rdfs:comment>
	<rdfs:comment xml:lang="zh-CN">项目的有关博客的URI。</rdfs:comment>
	<rdfs:domain rdf:resource="http://usefulinc.com/ns/doap#Project" />
	<rdfs:range rdf:resource="http://www.w3.org/2000/01/rdf-schema#Resource" />
    <rdfs:range rdf:resource="http://rdfs.org/sioc/types#Weblog" />
</rdf:Property>

</rdf:RDF>

